LambdaS5/coq/LjsAuxiliary.v
@@ -1,6 +1,22 @@
 Generalizable All Variables.
 Set Implicit Arguments.
 Require Import LjsShared.
+Require Import JsNumber.
 Require Import Utils.
 Require Import LjsSyntax.
+Require Import LjsPrettyInterm LjsPrettyRules LjsPrettyRulesIndexed.
+Require Import LjsCompleteness.
 
+Implicit Type A B : Type.
+Implicit Type st : store.
+Implicit Type e : expr.
+Implicit Type v : value.
+Implicit Type s : string.
+Implicit Type n : number.
+Implicit Type i : id.
+Implicit Type o : out.
+Implicit Type c : ctx.
+Implicit Type ptr : object_ptr.
+Implicit Type obj : object.
+Implicit Type re : result.
+Implicit Type r : res.
