LambdaS5/coq/LjsSyntaxAux.v
@@ -14,3 +14,20 @@ Global Instance value_inhab : Inhab value.
 Proof.
     intros. apply (prove_Inhab value_undefined).
 Qed.
+
+Inductive pure_expr : ctx -> expr -> Prop :=
+| pure_expr_empty : forall c, pure_expr c expr_empty
+| pure_expr_null : forall c, pure_expr c expr_null
+| pure_expr_undefined : forall c, pure_expr c expr_undefined
+| pure_expr_string : forall c s, pure_expr c (expr_string s)
+| pure_expr_number : forall c n, pure_expr c (expr_number n)
+| pure_expr_true : forall c, pure_expr c expr_true
+| pure_expr_false : forall c, pure_expr c expr_false
+| pure_expr_id : forall c i, index c i -> pure_expr c (expr_id i)
+| pure_expr_if : forall c e1 e2 e3, 
+    pure_expr c e1 -> pure_expr c e2 -> pure_expr c e3 -> 
+    pure_expr c (expr_if e1 e2 e3)
+| pure_expr_seq : forall c e1 e2, 
+    pure_expr c e1 -> pure_expr c e2 ->
+    pure_expr c (expr_seq e1 e2)
+.
